src/tactic/vampire/rr.pl
@@ -2,6 +2,577 @@
 
 :- initialization(main, main).
 
+mat(Stk, ["nl" | Tks], Mat) :-
+  mat([[] | Stk], Tks, Mat).
+
+mat([Num | Stk], ["y" | Tks], Mat) :-
+  mat([sym(Num) | Stk], Tks, Mat).
+
+mat([Trm | Stk], ["ng" | Tks], Mat) :-
+  mat([neg(Trm) | Stk], Tks, Mat).
+
+mat([Trm | Stk], ["ps" | Tks], Mat) :-
+  mat([pos(Trm) | Stk], Tks, Mat).
+
+mat([Hd, Tl | Stk], ["cs" | Tks], Mat) :-
+  mat([[Hd | Tl] | Stk], Tks, Mat).
+
+mat(Stk, [NumStr | Tks], Mat) :-
+  number_string(Num, NumStr),
+  mat([Num | Stk], Tks, Mat).
+
+mat([Mat], [], Mat).
+
+join_string([], _, "").
+
+join_string([Str], _, Str).
+
+join_string([Str | Strs], Jn, Rst) :-
+  string_concat(Str, Jn, Str1),
+  join_string(Strs, Jn, Str2),
+  string_concat(Str1, Str2, Rst).
+
+join_string(Strs, Str) :-
+  join_string(Strs, "", Str).
+
+tptp_trm(sym(Num), Num, []).
+
+tptp_trm(sym(Num), Str) :-
+  number_string(Num, NumStr),
+  string_concat("s", NumStr, Str).
+
+tptp_trm(app(Trm1, Trm2), Rst) :-
+  tptp_trm(Trm1, Num, Strs),
+  number_string(Num, NumStr),
+  tptp_trm(Trm2, Str),
+  append(Strs, [Str], ArgStrs),
+  join_string(ArgStrs, ", ", ArgsStr),
+  join_string(["s", NumStr, "(", ArgsStr, ")"], Rst).
+
+tptp_lit(neg(Trm), Str) :-
+  tptp_trm(Trm, Tmp),
+  string_concat("~ " , Tmp, Str).
+
+tptp_lit(pos(Trm), Str) :-
+  tptp_trm(Trm, Str).
+
+tptp_cla(Cla, Idx, Str) :-
+  number_string(Idx, IdxStr),
+  maplist(tptp_lit, Cla, Tmp),
+  join_string(Tmp, " | ", Bdy),
+  join_string(["cnf(c", IdxStr,
+    ", negated_conjecture, (", Bdy, "))."], Str).
+
+tptp_mat([Cla], Idx, Str) :-
+  tptp_cla(Cla, Idx, Str).
+
+tptp_mat([Cla | Mat], Idx, Str) :-
+  tptp_cla(Cla, Idx, ClaStr),
+  NewIdx is Idx + 1,
+  tptp_mat(Mat, NewIdx, MatStr),
+  join_string([ClaStr, " ", MatStr], Str).
+
+temp_loc("/var/tmp/temp_goal_file").
+
+write_goal(Goal) :-
+  temp_loc(Loc),
+  open(Loc, write, Stream),
+  write(Stream, Goal),
+  close(Stream).
+
+vampire(Strs) :-
+  temp_loc(Loc),
+  setup_call_cleanup(
+    process_create(
+      path(vampire),
+      ["--avatar", "off", Loc],
+      [stdout(pipe(Out))]
+    ),
+    read_lines(Out, Strs),
+    close(Out)
+  ).
+
+read_lines(Out, []) :-
+  read_line_to_string(Out, end_of_file), !.
+
+read_lines(Out, Cdss) :-
+  read_line_to_codes(Out, Cds),
+  read_lines(Cds, Out, Cdss).
+
+read_lines(end_of_file, _, []) :- !.
+
+read_lines(Cds, Out, [Cds | Cdss]) :-
+        read_line_to_codes(Out, Tmp),
+        read_lines(Tmp, Out, Cdss).
+
+foo('foo') :- true.
+
+is_digit(Cd) :- 47 < Cd, Cd < 58.
+
+head_is_digit([Cd | _]) :- is_digit(Cd).
+
+parse_rul("input", inp).
+
+parse_rul(Str, res(Idx1, Idx2)) :-
+  ( string_concat("resolution ", Tmp, Str) ;
+    string_concat("subsumption resolution ", Tmp, Str) ),
+  split_string(Tmp, ",", "", [NumStr1, NumStr2]),
+  number_string(Num1, NumStr1),
+  Idx1 is Num1 - 1,
+  number_string(Num2, NumStr2),
+  Idx2 is Num2 - 1.
+
+split_string_at(Str, Sep, Fst, Snd) :-
+  string_concat(Fst, Tmp, Str),
+  string_concat(Sep, Snd, Tmp).
+
+parse_num(Acc, [Cd | Cds], Num, Rem) :-
+  is_digit(Cd),
+  parse_num([Cd | Acc], Cds, Num, Rem).
+
+parse_num(Acc, [Cd | Cds], Num, [Cd | Cds]) :-
+  not(is_digit(Cd)),
+  reverse(Acc, Tmp),
+  number_codes(Num, Tmp).
+
+parse_num(Str, Num, Rem) :-
+  string_codes(Str, Cds),
+  parse_num([], Cds, Num, Tmp),
+  string_codes(Rem, Tmp).
+
+parse_trm(Str, sym(Num), "") :-
+  string_concat("s", Tmp, Str),
+  number_string(Num, Tmp).
+
+parse_trm(Str, Trm, Rem) :-
+  string_concat("s", Tmp, Str),
+  split_string_at(Tmp, "(", Fst, Snd),
+  number_string(Num, Fst),
+  parse_trm(sym(Num), Snd, Trm, Rem).
+
+parse_trm(Trm, Str, Trm, Rem) :-
+  string_concat(")", Rem, Str).
+
+parse_trm(Acc, Str, Trm, Rem) :-
+  string_concat(", ", Tmp, Str),
+  parse_trm(Acc, Tmp, Trm, Rem).
+
+parse_trm(Acc, Str, Trm, Rem) :-
+  string_concat("X", Str1, Str),
+  parse_num(Str1, Num, Str2),
+  parse_trm(vpp(Acc, Num), Str2, Trm, Rem).
+
+parse_trm(Acc, Str, Trm, Rem) :-
+  parse_trm(Str, Arg, Tmp),
+  parse_trm(app(Acc, Arg), Tmp, Trm, Rem).
+
+parse_lit(Str, neg(Trm)) :-
+  string_concat("~", Tmp, Str),
+  parse_trm(Tmp, Trm, "").
+
+parse_lit(Str, pos(Trm)) :-
+  parse_trm(Str, Trm, "").
+
+parse_cla("$false", []) :- !.
+
+parse_cla(Str, Cla) :-
+  split_string(Str, "|", " ", LitStrs),
+  maplist(parse_lit, LitStrs, Cla).
+
+parse_line(Cds, line(Idx, Cla, Rul)) :-
+  string_codes(Str, Cds),
+  split_string(Str, ".[", "] ", [NumStr, ClaStr, RulStr]),
+  number_string(Num, NumStr),
+  Idx is Num - 1,
+  parse_cla(ClaStr, Cla),
+  parse_rul(RulStr, Rul).
+
+read_proof(Lns) :-
+  vampire(Cds),
+  include(head_is_digit, Cds, Tmp),
+  maplist(parse_line, Tmp, Lns).
+
+compile(Mat, Lns, Num, Infs, Rst) :-
+  member(line(Num, Tgt, Rul), Lns),
+  compile(Mat, Lns, Num, Tgt, Rul, Infs, Rst).
+
+max(Num1, Num2, Num1) :- Num1 >= Num2.
+max(Num1, Num2, Num2) :- Num1 < Num2.
+
+fresh_var(sym(_), 0).
+
+fresh_var(app(Trm1, Trm2), Num) :-
+  fresh_var(Trm1, Num1),
+  fresh_var(Trm2, Num2),
+  max(Num1, Num2, Num).
+
+fresh_var(vpp(Trm1, Idx), Num) :-
+  fresh_var(Trm1, Num1),
+  Num2 is Idx + 1,
+  max(Num1, Num2, Num).
+
+fresh_var(neg(Trm), Num) :-
+  fresh_var(Trm, Num).
+
+fresh_var(pos(Trm), Num) :-
+  fresh_var(Trm, Num).
+
+fresh_var(Cla, Num) :-
+  maplist(fresh_var, Cla, Nums),
+  max_list(Nums, Num).
+
+offset(Ofs, Src, map(Src, Tgt)) :-
+  Tgt is Src + Ofs.
+
+union([], []).
+
+union([Lst | Lsts], Un) :-
+  union(Lsts, Tmp),
+  union(Lst, Tmp, Un).
+
+vars(sym(_), []).
+
+vars(app(Trm1, Trm2), Nums) :-
+  vars(Trm1, Nums1),
+  vars(Trm2, Nums2),
+  union(Nums1, Nums2, Nums).
+
+vars(vpp(Trm, Num), Nums) :-
+  vars(Trm, Tmp),
+  union([Num], Tmp, Nums).
+
+vars(neg(Trm), Nums) :-
+  vars(Trm, Nums).
+
+vars(pos(Trm), Nums) :-
+  vars(Trm, Nums).
+
+vars(Cla, Nums) :-
+  maplist(vars, Cla, Numss),
+  union(Numss, Nums).
+
+disjoiner(Cla1, Cla2, Dsj) :-
+  fresh_var(Cla1, Num),
+  vars(Cla2, Nums),
+  maplist(offset(Num), Nums, Dsj).
+
+rot(0, [Hd | Tl], [Hd | Tl]).
+
+rot(Idx, [Hd | Tl], [NewHd, Hd | NewTl]) :-
+  rot(NewIdx, Tl, [NewHd | NewTl]),
+  Idx is NewIdx + 1.
+
+% rot_core([Lit | Cla], 0, Lit, Cla).
+%
+% rot_core([Lit1 | Cla1], Num, Lit2, [Lit1 | Cla2]) :-
+%   rot_core(Cla1, Tmp, Lit2, Cla2),
+%   Num is Tmp + 1.
+%
+% rot(Cla, [num(Num), rot], [NewLit | NewCla]) :-
+%   rot_core(Cla, Num, NewLit, NewCla).
+
+subst(_, sym(Num), sym(Num)).
+
+subst(Maps, app(Trm1, Trm2), app(NewTrm1, NewTrm2)) :-
+  subst(Maps, Trm1, NewTrm1),
+  subst(Maps, Trm2, NewTrm2).
+
+subst(Maps, vpp(Trm, Num), vpp(NewTrm, NewNum)) :-
+  member(map(Num, NewNum), Maps), !,
+  number(NewNum),
+  subst(Maps, Trm, NewTrm).
+
+subst(Maps, vpp(Trm, Num), app(NewTrm1, NewTrm2)) :-
+  member(map(Num, NewTrm2), Maps), !,
+  not(number(NewTrm2)),
+  subst(Maps, Trm, NewTrm1).
+
+subst(Map, neg(Trm), neg(NewTrm)) :-
+  subst(Map, Trm, NewTrm).
+
+subst(Map, pos(Trm), pos(NewTrm)) :-
+  subst(Map, Trm, NewTrm).
+
+subst(Maps, Cla, NewCla) :-
+  maplist(subst(Maps), Cla, NewCla).
+
+trm_to_infs(sym(Num), [num(Num), sym]).
+
+trm_to_infs(app(Trm1, Trm2), Infs) :-
+  trm_to_infs(Trm1, Infs1),
+  trm_to_infs(Trm2, Infs2),
+  append([Infs1, Infs2, [app]], Infs).
+
+trm_to_infs(vpp(Trm, Num), Infs) :-
+  trm_to_infs(Trm, Tmp),
+  append(Tmp, [num(Num), vpp], Infs).
+
+map_to_infs(map(Src, Tgt), [num(Src), num(Tgt)]) :-
+  number(Tgt).
+
+map_to_infs(map(Num, Trm), [num(Num) | Infs]) :-
+  trm_to_infs(Trm, Infs).
+
+maps_to_infs([], [nil]).
+
+maps_to_infs([Map | Maps], Infs) :-
+  maps_to_infs(Maps, Infs1),
+  map_to_infs(Map, Infs2),
+  append([Infs1, Infs2, [cons]], Infs).
+
+% compose_map(Maps, Src, Tgt, map(Src, NewTgt)) :-
+%   member(map(Tgt, NewTgt), Maps), !.
+%
+% compose_map(Maps, Src, Tgt, map(Src, Tgt)) :-
+%   not(member(map(Tgt, _), Maps)).
+%
+
+substitutee(Src, map(Src, _)).
+
+compose_maps([], Maps, Maps).
+
+compose_maps([map(Src, Tgt) | Maps1], Maps2, [map(Src, NewTgt) | NewMaps]) :-
+  subst(Maps2, Tgt, NewTgt),
+  exclude(substitutee(Src), Maps2, NewMaps2),
+  compose_maps(Maps1, NewMaps2, NewMaps).
+
+%compose_maps(Maps1, [map(Src, Tgt) | Maps2], [NewMap | NewMaps]) :-
+%  compose_map(Maps1, Src, Tgt, NewMap),
+%  compose_maps(Maps1, Maps2, NewMaps).
+
+unifier(sym(Num), sym(Num), []).
+
+unifier(app(Trm1, Trm2), app(Trm3, Trm4), Maps) :-
+  unifier(Trm2, Trm4, Maps2),
+  subst(Maps2, Trm1, NewTrm1),
+  subst(Maps2, Trm3, NewTrm3),
+  unifier(NewTrm1, NewTrm3, Maps1),
+  compose_maps(Maps1, Maps2, Maps).
+
+unifier(app(Trm1, Trm2), vpp(Trm3, Num), Maps) :-
+  vars(Trm2, Nums),
+  not(member(Num, Nums)),
+  subst([map(Num, Trm2)], Trm1, NewTrm1),
+  subst([map(Num, Trm2)], Trm3, NewTrm3),
+  unifier(NewTrm1, NewTrm3, TmpMaps),
+  compose_maps([map(Num, Trm2)], TmpMaps, Maps).
+
+unifier(vpp(Trm1, Num), app(Trm2, Trm3), Maps) :-
+  vars(Trm3, Nums),
+  not(member(Num, Nums)),
+  subst([map(Num, Trm1)], Trm1, NewTrm1),
+  subst([map(Num, Trm2)], Trm2, NewTrm2),
+  unifier(NewTrm1, NewTrm2, TmpMaps),
+  compose_maps([map(Num, Trm3)], TmpMaps, Maps).
+
+unifier(vpp(Trm1, Num1), vpp(Trm2, Num2), Maps) :-
+  subst([map(Num2, Num1)], Trm1, NewTrm1),
+  subst([map(Num2, Num1)], Trm2, NewTrm2),
+  unifier(NewTrm1, NewTrm2, TmpMaps),
+  compose_maps([map(Num2, Trm1)], TmpMaps, Maps).
+
+unifiers(Trm1, Trm2, Dsj, Unf1, Unf2) :-
+  subst(Dsj, Trm2, NewTrm2),
+  unifier(Trm1, NewTrm2, Unf1),
+  compose_maps(Dsj, Unf1, Unf2).
+
+compile_res(Infs1, [neg(Trm1) | Cla1], Infs2, [pos(Trm2) | Cla2], Infs, Rst) :-
+  disjoiner([neg(Trm1) | Cla1], [pos(Trm2) | Cla2], Dsj),
+  unifiers(Trm1, Trm2, Dsj, Unf1, Unf2),
+  subst(Unf1, Cla1, NewCla1),
+  subst(Unf2, Cla2, NewCla2),
+  maps_to_infs(Unf1, MapInfs1),
+  maps_to_infs(Unf2, MapInfs2),
+  append([Infs1, MapInfs1, [sub], Infs2, MapInfs2, [sub, res]], Infs),
+  append(NewCla1, NewCla2, Rst).
+
+range(0, Acc, Acc).
+
+range(Num, Acc, Nums) :-
+  0 < Num,
+  NewNum is Num - 1,
+  range(NewNum, [NewNum | Acc], Nums).
+
+range(Num, Nums) :-
+  range(Num, [], Nums).
+
+member_rev(Lst, Elm) :- member(Elm, Lst).
+
+merge_instantiators([], Inst, Inst).
+
+merge_instantiators([map(Idx, Tgt) | Inst1], Inst2, Inst) :-
+  member(map(Idx, Tgt), Inst2),
+  merge_instantiators(Inst1, Inst2, Inst).
+
+merge_instantiators([map(Idx, Tgt) | Inst1], Inst2, [map(Idx, Tgt) | Inst]) :-
+  not(member(map(Idx, _), Inst2)),
+  merge_instantiators(Inst1, Inst2, Inst).
+
+instantiator(sym(Num), sym(Num), []).
+
+instantiator(app(Trm1, Trm2), app(Trm3, Trm4), Maps) :-
+  instantiator(Trm1, Trm3, Maps1),
+  instantiator(Trm2, Trm4, Maps2),
+  merge_instantiators(Maps1, Maps2, Maps).
+
+instantiator(vpp(Trm1, Num), app(Trm2, Trm3), Maps) :-
+  instantiator(Trm1, Trm2, Maps1),
+  merge_instantiators(Maps1, [map(Num, Trm3)], Maps).
+
+instantiator(vpp(Trm1, Num1), vpp(Trm2, Num2), Maps) :-
+  instantiator(Trm1, Trm2, Maps1),
+  merge_instantiators(Maps1, [map(Num1, Num2)], Maps).
+
+instantiator(neg(Src), neg(Tgt), Maps) :-
+  instantiator(Src, Tgt, Maps).
+
+instantiator(pos(Src), pos(Tgt), Maps) :-
+  instantiator(Src, Tgt, Maps).
+
+choose_map([], _, [], []).
+
+choose_map([Lit | Cla], Tgt, Maps, [LitNum | ClaNums]) :-
+  nth0(LitNum, Tgt, TgtLit),
+  instantiator(Lit, TgtLit, LitMaps),
+  choose_map(Cla, Tgt, ClaMaps, ClaNums),
+  merge_instantiators(LitMaps, ClaMaps, Maps).
+
+surjective(Ran, Nums) :-
+  length(Ran, Lth),
+  range(Lth, Idxs),
+  subset(Idxs, Nums).
+
+% increment(Num, SuccNum) :-
+%   SuccNum is Num + 1.
+
+% find_indices(_, [], []).
+%
+% find_indices(Elm, [Elm | Lst], [0 | Idxs]) :-
+%   find_indices(Elm, Lst, Tmp),
+%   maplist(increment, Tmp, Idxs).
+%
+% find_indices(Elm, [Hd | Lst], Idxs) :-
+%   not(Elm = Hd),
+%   find_indices(Elm, Lst, Tmp),
+%   maplist(increment, Tmp, Idxs).
+
+count(_, [], 0).
+
+count(Elm, [Elm | Lst], Cnt) :-
+  count(Elm, Lst, Tmp),
+  Cnt is Tmp + 1.
+
+count(Elm, [Hd | Lst], Cnt) :-
+  not(Elm = Hd),
+  count(Elm, Lst, Cnt).
+
+compile_cnts_aux(Cla, Idx, Tl, [], Cla, Tl) :-
+  not(member(Idx, Tl)).
+
+compile_cnts_aux(Cla, Idx, Tl, [num(Num), rot, cont | Infs], RstCla, RstTl) :-
+  nth0(PredNum, Tl, Idx),
+  Num is PredNum + 1,
+  rot(PredNum, Tl, [Idx | NewTl]),
+  rot(Num, Cla, NewCla),
+  compile_cnts_aux(NewCla, Idx, NewTl, Infs, RstCla, RstTl).
+
+compile_cnts(Cla, Idx, Idxs, [], Cla) :-
+  not(member(Idx, Idxs)).
+
+compile_cnts(Cla, Idx, Idxs, Infs, Rst) :-
+  count(Idx, Idxs, 1),
+  NewIdx is Idx + 1,
+  compile_cnts(Cla, NewIdx, Idxs, Infs, Rst).
+
+compile_cnts(Cla, Idx, Idxs, [num(Fst), rot | Infs], Rst) :-
+  count(Idx, Idxs, Cnt),
+  1 < Cnt,
+  nth0(Fst, Idxs, Idx),
+  rot(Fst, Idxs, [Idx | Idxs1]),
+  rot(Fst, Cla, Cla1),
+  compile_cnts_aux(Cla1, Idx, Idxs1, Infs1, Cla2, Idxs2),
+  SuccIdx is Idx + 1,
+  compile_cnts(Cla2, SuccIdx, [Idx | Idxs2], Infs2, Rst),
+  append(Infs1, Infs2, Infs).
+
+compile_cnts(Cla, Idxs, Infs, Rst) :-
+   compile_cnts(Cla, 0, Idxs, Infs, Rst).
+
+compute_maps(Cla, Tgt, Maps, Nums) :-
+  choose_map(Cla, Tgt, Maps, Nums),
+  surjective(Tgt, Nums).
+
+compile_map([], [], [], []).
+
+compile_map(Cla, Tgt, Infs, Rst) :-
+  disjoiner(Tgt, Cla, Dsj),
+  subst(Dsj, Cla, Cla1),
+  compute_maps(Cla1, Tgt, Inst, Nums),
+  subst(Inst, Cla1, Cla2),
+  compose_maps(Dsj, Inst, Maps),
+  maps_to_infs(Maps, MapInfs),
+  compile_cnts(Cla2, Nums, CntInfs, Rst),
+  append(MapInfs, [sub | CntInfs], Infs).
+
+compile(Mat, _, Num, Tgt, inp, [num(Num), hyp | Infs], Rst) :-
+  nth0(Num, Mat, Cla),
+  compile_map(Cla, Tgt, Infs, Rst).
+
+compile(Mat, Lns, _, Tgt, res(Num1, Num2), Infs, Rst) :-
+  compile(Mat, Lns, Num1, Tmp1, Rst1),
+  compile(Mat, Lns, Num2, Tmp2, Rst2),
+  rot(Idx1, Rst1, Cla1),
+  rot(Idx2, Rst2, Cla2),
+  append(Tmp1, [num(Idx1), rot], Infs1),
+  append(Tmp2, [num(Idx2), rot], Infs2),
+  ( compile_res(Infs1, Cla1, Infs2, Cla2, ResInfs, Tmp) ;
+    compile_res(Infs2, Cla2, Infs1, Cla1, ResInfs, Tmp) ),
+  compile_map(Tmp, Tgt, MapInfs, Rst),
+  append(ResInfs, MapInfs, Infs).
+
+compile(_, _, _, _, res(Num1, Num2), resfail(Num1, Num2), _).
+
+compile(Mat, Lns, _, Tgt, map(Num), Infs, Rst) :-
+  compile(Mat, Lns, Num, Infs1, Tmp),
+  compile_map(Tmp, Tgt, Infs2, Rst),
+  append(Infs1, Infs2, Infs).
+
+filter_infs([], []).
+
+filter_infs([nil, sub | Infs], Rst) :-
+  filter_infs(Infs, Rst).
+
+filter_infs([num(0), rot | Infs], Rst) :-
+  filter_infs(Infs, Rst).
+
+filter_infs([Inf | Infs], [Inf | Rst]) :-
+  filter_infs(Infs, Rst).
+
+compile(Mat, Lns, Infs) :-
+  length(Lns, Lth),
+  Idx is Lth - 1,
+  nth0(Idx, Lns, line(Num, [], Rul)),
+  compile(Mat, Lns, Num, [], Rul, TmpInfs, _),
+  filter_infs(TmpInfs, Infs).
+
+format_infs(num(Num), Str) :-
+  number_string(Num, Str).
+format_infs(hyp, "h").
+format_infs(res, "r").
+format_infs(rot, "t").
+format_infs(cont, "c").
+format_infs(sub, "s").
+
+print_infs(Infs) :-
+  maplist(format_infs, Infs, Strs),
+  join_string(Strs, " ", Str),
+  write(Str).
+
 main([Argv]) :-
   split_string(Argv, " ", " ", Tks),
-  print(Tks).
+  mat([], Tks, Mat),
+  tptp_mat(Mat, 1, Goal),
+  write_goal(Goal),
+  read_proof(Lns),
+  compile(Mat, Lns, Infs),
+  print_infs(Infs).
