src/tactic/vampire/vampire.sh
@@ -1,7 +1,5 @@
 #!/bin/sh
 
-# echo $1 > $2
+echo $1 > $2
 
-# vampire --avatar off $2
-
-echo "Hello!"
+vampire --avatar off $2
